veric/seplog.v
@@ -564,7 +564,7 @@ Definition funspecs_assert (FunSpecs: Maps.PTree.t funspec): assert :=
  assert_of (fun rho =>
    □ ((∀ id: ident, ∀ fs:funspec,  ⌜FunSpecs!!id = Some fs⌝ →
             ∃ b:block,⌜Map.get (ge_of rho) id = Some b⌝ ∧ func_at fs (b,0)) ∧
-     (∀ fs b, ⌜∀ id, Map.get (ge_of rho) id = Some b → FunSpecs!!id = Some fs⌝ →
+      (∀ b, ⌜∃ id, Map.get (ge_of rho) id = Some b ∧ FunSpecs!!id = None⌝ →
             mapsto_no (b, 0) Share.bot))).
 
 Definition globals_only (rho: environ) : environ := (mkEnviron (ge_of rho) (Map.empty _) (Map.empty _)).
@@ -605,8 +605,8 @@ assert (forall FS FS' rho,
 { intros. rewrite /funspecs_assert.
   iIntros "#(H1 & H2) !>"; iSplit.
   - iIntros (??); rewrite -H //.
-  - iIntros (???); iApply "H2".
-    iPureIntro; intros; rewrite H; eauto. }
+  - iIntros (? (? & ? & HF)); rewrite -H in HF.
+    iApply "H2"; eauto. }
 split=> rho; iSplit; iApply H; auto.
 Qed.
 
